next_t_loop_view

crypto_examples/mulntt_ct/mulntt_ct.dfy
@@ -1,6 +1,6 @@
 include "mulntt_ct_rec.dfy"
 
-module ntt {
+module mulntt_ct {
     import opened Seq
     import opened Power
     import opened Power2
@@ -12,127 +12,11 @@ module ntt {
     import opened ntt_index
 
     import opened mulntt_ct_rec
-    // import opened ntt_recs
-    // import opened rindex
-    // import opened bins
-    import opened polys
+    import opened ntt_polys
 
+    // function method A(): n_sized
 
-    function method A(): n_sized
-
-    function method P(): n_sized
-
-    // lemma A_table_index_bounded_lemma(s: nat, d: pow2_t, j: nat, t: pow2_t)
-    //     requires 0 <= d.exp < LOGN;
-    //     requires 0 <= t.exp < LOGN;
-    //     requires block_count(t) == 2 * d.full;
-    //     // requires block_count(pow2_double(t)) == d.full;
-    //     requires j < t.full;
-    //     requires s < (2 * d.full) * j + d.full;
-    //     ensures s + d.full < N;
-    // {
-    //     assume false;
-    //     // block_count_product_lemma(t);
-    //     // assert block_count(t) * t.full == N;
-    // }
-
-    // datatype slice_loop_view = slice_loop_view(
-    //     lower: lpolys,
-    //     higher: lpolys)
-    // {
-    //     predicate slice_view_wf()
-    //     {
-    //         && higher.level_wf()
-    //         && lower.level_wf()
-    //         && 1 <= higher.bsize.exp <= LOGN
-    //         && higher.build_smaller_level() == lower
-    //     }
-
-    //     function get_even_poly(which: nat): (r: seq<elem>)
-    //         requires slice_view_wf();
-    //         requires which < |higher.blocks|;
-    //         ensures |higher.blocks[which]| == higher.bsize.full;
-    //         ensures r == even_indexed_items(higher.blocks[which], higher.bsize);
-    //     {
-    //         higher.level_index_correspondence_lemma(which, lower);
-    //         lower.blocks[2 * which]
-    //     }
-
-    //     function get_odd_poly(which: nat): (r: seq<elem>)
-    //         requires slice_view_wf();
-    //         requires which < |higher.blocks|;
-    //         ensures |higher.blocks[which]| == higher.bsize.full;
-    //         ensures r == odd_indexed_items(higher.blocks[which], higher.bsize);
-    //     {
-    //         higher.level_index_correspondence_lemma(which, lower);
-    //         lower.blocks[2 * which + 1]
-    //     }
-
-    //     predicate slice_view_inv(a: seq_ j: nat)
-    //     {
-    //         // && forall i | 0 <= i < |lower
-    //         //      block_eval_inv(, lower.block[i], bsize, k)
-
-    //     }
-    // }
-
-
-    // method slice_loop(
-    //     a: n_sized,
-    //     u: nat,
-    //     d: pow2_t,
-    //     w: elem,
-    //     ghost j: nat,
-    //     ghost t: pow2_t,
-    //     ghost sv: slice_loop_view)
-
-    // returns (new_a: n_sized)
-    
-    // // ghost new_blocks: seq<seq<elem>>)
-    //     // requires |blocks| == d.full;
-    //     requires 0 <= t.exp < LOGN;
-    //     requires 0 <= d.exp < LOGN;
-
-    //     requires 2 * d.full * bit_rev_int(j, t) >= 0;
-
-    //     requires block_count(t) == 2 * d.full;
-    //     // d blocks, each of 2t size 
-    //     // requires block_count(pow2_double(t)) == d.full;
-    //     requires j < t.full;
-    //     requires u == (2 * d.full) * j;
-
-    //     requires sv.slice_view_wf();
-    //     // requires t.exp == 0 ==> a == A(); // not quite right
-
-    //     // ensures |new_blocks| == d.full;
-    // {
-    //     var s := u;
-    //     // new_blocks := blocks;
-    //     new_a := a;
-
-    //     assume w == modpow(PSI, 2 * d.full * bit_rev_int(j, t) + d.full);
-
-    //     while (s < u + d.full)
-    //         // invariant |new_blocks| == |blocks|;
-    //         // invariant 
-    //     {
-    //         A_table_index_bounded_lemma(s, d, j, t);
-    //         ghost var b_idx := s - u;
-    //         var e := a[s];
-    //         var o := a[s + d.full];
-
-    //         var xe = (pow(OMEGA, d * bit_rev_int(2*j, logn), Q) * pow(PSI, d, Q)) % Q;
-
-    //         // assume e == ;
-
-    //         var x := modmul(o, w);
-    //         new_a := new_a[s+d.full := modsub(e, x)];
-    //         new_a := new_a[s := modadd(e, x)];
-
-    //         s := s + 1;
-    //         // new_blocks := new_blocks[b_idx := blocks[b_idx]];
-    //     }
-    // }
+    // function method P(): n_sized
 
     // lemma P_table_index_bounded_lemma(t: pow2_t, j: nat)
     //     requires t.exp < LOGN;
@@ -142,42 +26,68 @@ module ntt {
     //     assume false;
     // }
 
-    // method level_loop(a: n_sized, t: pow2_t, d: pow2_t)
-    //     requires t.exp < LOGN;
-    //     requires d.exp + 1 + t.exp == LOGN;
-    //     requires block_count(pow2_double(t)) == d.full;
-    //     requires block_count(t) == 2 * d.full;
-    // {
-    //     var j := 0;
-    //     var u := 0;
+    method j_loop(a: n_sized, d: pow2_t, j: nat, ghost view: loop_view)
+    returns (a': n_sized)
 
-    //     ghost var blocks := seq(d.full, n requires 0 <= n < d.full => []);
+        requires view.j_loop_inv(a, d, j);
+        requires j < view.lsize().full;
+        ensures view.j_loop_inv(a', d, j + 1);
+    {
+        view.s_loop_inv_pre_lemma(a, d, j);
 
-    //     while (j < t.full)
-    //         invariant 0 <= u == (2 * d.full) * j;
-    //         invariant |blocks| == d.full;
-    //     {
-    //         P_table_index_bounded_lemma(t, j);
-    //         var w := P()[t.full + j]; // psi_t * w_t^bitrev(j)
+        var u := (2 * j) * d.full;
+        var w := x_value(2 * j, d); // TODO: read from table
+        // P_table_index_bounded_lemma(t, j);
+        // var w := P()[t.full + j]; // psi_t * w_t^bitrev(j)
 
-    //         ghost var prev_u := u;
-    //         ghost var prev_j := j;
+        var s := u;
+        a' := a;
 
-    //         blocks := slice_loop(u, d, w, j, t, blocks);
-    //         j := j + 1;
-    //         u := u + 2 * d.full;
+        ghost var bi := 0;
 
-    //         calc == {
-    //             u;
-    //             prev_u + 2 * d.full;
-    //             2 * d.full * prev_j + 2 * d.full;
-    //             {
-    //                 LemmaMulIsDistributive(2 * d.full, prev_j, 1);
-    //             }
-    //             (2 * d.full) * (prev_j + 1);
-    //         }
-    //     }
-    // }
+        while (s < u + d.full)
+            invariant view.s_loop_inv(a', d, j, s-u);
+        {
+            var a :n_sized := a';
+            var bi := s-u;
+
+            var _ := view.higher_points_view_index_lemma(a, d, j, bi);
+
+            var e := a[s];
+            var o := a[s + d.full];
+
+            var x := modmul(o, w);
+            a' := a[s+d.full := modsub(e, x)];
+            a' := a'[s := modadd(e, x)];
+            s := s + 1;
+
+            view.s_loop_inv_peri_lemma(a, a', d, j, bi);
+        }
+
+        assert s == u + d.full;
+        view.s_loop_inv_post_lemma(a', d, j, d.full);
+    }
+
+    method t_loop(a: n_sized, t: pow2_t, d: pow2_t, ghost view: loop_view)
+        returns (a': n_sized)
+
+        requires view.j_loop_inv(a, d, 0);
+        requires t == view.lsize();
+        // requires t.exp < LOGN;
+        // requires d.exp + 1 + t.exp == LOGN;
+        // requires block_count(pow2_double(t)) == d.full;
+        // requires block_count(t) == 2 * d.full;
+    {
+        var j := 0;
+        a' := a;
+
+        while (j < t.full)
+            invariant view.j_loop_inv(a', d, j);
+        {
+            a' := j_loop(a', d, j, view);
+            j := j + 1;
+        }
+    }
 
     // method mulntt_ct()
     // {
@@ -198,7 +108,7 @@ module ntt {
 
     //         // assert d.exp + 1 + t.exp == LOGN;
     //         // assume d.full * 2 * t.full == N;
-    //         level_loop(t, d);
+    //         j_loop(t, d);
     //         t := pow2_double(t);
     //         // block_count_half_lemma(t);
     //     }
